LowParse.Low.ConstInt32 validator fast

src/lowparse/LowParse.Low.ConstInt32.fst
@@ -10,6 +10,7 @@ include LowParse.Low.Combinators
 include LowParse.Low.BoundedInt
 
 module U32 = FStar.UInt32
+module U8 = FStar.UInt8
 module HS = FStar.HyperStack
 module HST = FStar.HyperStack.ST
 module B = LowStar.Buffer
@@ -29,6 +30,7 @@ let valid_constint32le
   valid_facts (parse_int32_le ()) h input pos;
   parse_constint32le_unfold v (bytes_of_slice_from h input pos)
 
+inline_for_extraction
 let read_int32_le : (leaf_reader (parse_int32_le ()))
 = make_total_constant_size_reader 4 4ul decode_int32_le (decode_int32_le_total_constant ()) (fun #rrel #rel b pos ->
     let h = HST.get () in
@@ -40,7 +42,7 @@ let read_int32_le : (leaf_reader (parse_int32_le ()))
     Cast.uint8_to_uint32 r0 `U32.add` (256ul `U32.mul` (Cast.uint8_to_uint32 r1 `U32.add` (256ul `U32.mul` (Cast.uint8_to_uint32 r2 `U32.add` (256ul `U32.mul` Cast.uint8_to_uint32 r3)))))
   )
 
-
+inline_for_extraction
 let validate_constint32le_slow
   (v: U32.t { 0 <= U32.v v /\ U32.v v < 4294967296 } )
 : Tot (validator (parse_constint32le (U32.v v)))
@@ -60,3 +62,176 @@ let validate_constint32le_slow
     else
       validator_error_generic
 
+inline_for_extraction
+let read_constint32le 
+  (v: U32.t { 0 <= U32.v v /\ U32.v v < 4294967296 } )
+: Tot (leaf_reader (parse_constint32le (U32.v v)))
+= fun #rrel #rel input pos ->
+    v
+
+inline_for_extraction
+let decompose_int32_le_0
+  (v: nat { 0 <= v /\ v < 4294967296 } )
+: Tot (b0: nat { 0 <= b0 /\ b0 < 256 } )
+= v % 256
+
+inline_for_extraction
+let decompose_int32_le_1
+  (v: nat { 0 <= v /\ v < 4294967296 } )
+: Tot (b1: nat { 0 <= b1 /\ b1 < 256 } )
+= v / 256 % 256
+
+inline_for_extraction
+let decompose_int32_le_2
+  (v: nat { 0 <= v /\ v < 4294967296 } )
+: Tot (b2: nat { 0 <= b2 /\ b2 < 256 } )
+= v / 65536 % 256
+
+inline_for_extraction
+let decompose_int32_le_3
+  (v: nat { 0 <= v /\ v < 4294967296 } )
+: Tot (b3: nat { 0 <= b3 /\ b3 < 256 } )
+= v / 16777216
+
+let compose_int32_le
+  (b0: nat { 0 <= b0 /\ b0 < 256 } )
+  (b1: nat { 0 <= b1 /\ b1 < 256 } )
+  (b2: nat { 0 <= b2 /\ b2 < 256 } )
+  (b3: nat { 0 <= b3 /\ b3 < 256 } )
+: Tot (v: nat { 0 <= v /\ v < 4294967296 } ) 
+= b0 
+  + 256 `FStar.Mul.op_Star` (b1
+  + 256 `FStar.Mul.op_Star` (b2
+  + 256 `FStar.Mul.op_Star` b3))
+
+let decompose_compose_equiv
+  (v: nat { 0 <= v /\ v < 4294967296 } )
+: Lemma (compose_int32_le (decompose_int32_le_0 v) (decompose_int32_le_1 v) (decompose_int32_le_2 v) (decompose_int32_le_3 v) == v)
+= ()
+
+inline_for_extraction
+let compare_by_bytes
+  (a0: U8.t { 0 <= U8.v a0 /\ U8.v a0 < 256 } )
+  (a1: U8.t { 0 <= U8.v a1 /\ U8.v a1 < 256 } )
+  (a2: U8.t { 0 <= U8.v a2 /\ U8.v a2 < 256 } )
+  (a3: U8.t { 0 <= U8.v a3 /\ U8.v a3 < 256 } )
+  (b0: U8.t { 0 <= U8.v b0 /\ U8.v b0 < 256 } )
+  (b1: U8.t { 0 <= U8.v b1 /\ U8.v b1 < 256 } )
+  (b2: U8.t { 0 <= U8.v b2 /\ U8.v b2 < 256 } )
+  (b3: U8.t { 0 <= U8.v b3 /\ U8.v b3 < 256 } )
+= a0 = b0 && a1 = b1 && a2 = b2 && a3 = b3
+
+let compare_by_bytes'
+  (a0: U8.t { 0 <= U8.v a0 /\ U8.v a0 < 256 } )
+  (a1: U8.t { 0 <= U8.v a1 /\ U8.v a1 < 256 } )
+  (a2: U8.t { 0 <= U8.v a2 /\ U8.v a2 < 256 } )
+  (a3: U8.t { 0 <= U8.v a3 /\ U8.v a3 < 256 } )
+  (b0: U8.t { 0 <= U8.v b0 /\ U8.v b0 < 256 } )
+  (b1: U8.t { 0 <= U8.v b1 /\ U8.v b1 < 256 } )
+  (b2: U8.t { 0 <= U8.v b2 /\ U8.v b2 < 256 } )
+  (b3: U8.t { 0 <= U8.v b3 /\ U8.v b3 < 256 } )
+= (compose_int32_le (U8.v a0) (U8.v a1) (U8.v a2) (U8.v a3)) =
+  (compose_int32_le (U8.v b0) (U8.v b1) (U8.v b2) (U8.v b3))
+
+#push-options "--max_fuel 5 --z3rlimit 16"
+
+let compare_by_bytes_equiv
+  (a0: U8.t { 0 <= U8.v a0 /\ U8.v a0 < 256 } )
+  (a1: U8.t { 0 <= U8.v a1 /\ U8.v a1 < 256 } )
+  (a2: U8.t { 0 <= U8.v a2 /\ U8.v a2 < 256 } )
+  (a3: U8.t { 0 <= U8.v a3 /\ U8.v a3 < 256 } )
+  (b0: U8.t { 0 <= U8.v b0 /\ U8.v b0 < 256 } )
+  (b1: U8.t { 0 <= U8.v b1 /\ U8.v b1 < 256 } )
+  (b2: U8.t { 0 <= U8.v b2 /\ U8.v b2 < 256 } )
+  (b3: U8.t { 0 <= U8.v b3 /\ U8.v b3 < 256 } )
+: Lemma 
+  ((compare_by_bytes a0 a1 a2 a3 b0 b1 b2 b3) ==
+    compare_by_bytes' a0 a1 a2 a3 b0 b1 b2 b3)
+= let a = compose_int32_le (U8.v a0) (U8.v a1) (U8.v a2) (U8.v a3) in
+  let b = compose_int32_le (U8.v b0) (U8.v b1) (U8.v b2) (U8.v b3) in
+  decompose_compose_equiv a;
+  decompose_compose_equiv b
+
+#pop-options
+
+let decompose_compare
+  (v1 : nat { 0 <= v1 /\ v1 < 4294967296 } )
+  (v2 : nat { 0 <= v2 /\ v2 < 4294967296 } )
+: Lemma ( (v1 = v2) 
+    == (compare_by_bytes
+      (U8.uint_to_t (decompose_int32_le_0 v1))
+      (U8.uint_to_t (decompose_int32_le_1 v1))
+      (U8.uint_to_t (decompose_int32_le_2 v1))
+      (U8.uint_to_t (decompose_int32_le_3 v1))
+      (U8.uint_to_t (decompose_int32_le_0 v2))
+      (U8.uint_to_t (decompose_int32_le_1 v2))
+      (U8.uint_to_t (decompose_int32_le_2 v2))
+      (U8.uint_to_t (decompose_int32_le_3 v2))))
+= let a0 = U8.uint_to_t (decompose_int32_le_0 v1) in
+  let a1 = U8.uint_to_t (decompose_int32_le_1 v1) in
+  let a2 = U8.uint_to_t (decompose_int32_le_2 v1) in
+  let a3 = U8.uint_to_t (decompose_int32_le_3 v1) in
+  let b0 = U8.uint_to_t (decompose_int32_le_0 v2) in
+  let b1 = U8.uint_to_t (decompose_int32_le_1 v2) in
+  let b2 = U8.uint_to_t (decompose_int32_le_2 v2) in
+  let b3 = U8.uint_to_t (decompose_int32_le_3 v2) in
+  compare_by_bytes_equiv a0 a1 a2 a3 b0 b1 b2 b3;
+  decompose_compose_equiv v1;
+  decompose_compose_equiv v2
+
+
+#push-options " --max_fuel 5 --z3rlimit 16 "
+
+inline_for_extraction
+let inplace_compare
+  (v: U32.t { 0 <= U32.v v /\ U32.v v < 4294967296 } )
+  (#rrel: _)
+  (#rel: _)
+  (input: slice rrel rel)
+  (pos: U32.t)
+: HST.Stack bool
+  (requires (fun h -> valid (parse_int32_le ()) h input pos))
+  (ensures (fun h res h' -> 
+    B.modifies B.loc_none h h' /\
+    res == (U32.eq (contents (parse_int32_le ()) h input pos) v)))
+= let h = HST.get () in
+  let b = input.base in
+  [@inline_let] let _ = 
+    decode_int32_le_eq (Seq.slice (B.as_seq h b) (U32.v pos) (U32.v pos + 4));
+    decode_int32_le_total_constant ();
+    valid_facts (parse_int32_le ()) h input pos;
+    [@inline_let] let v' = contents (parse_int32_le ()) h input pos in
+    decompose_compose_equiv (U32.v v);
+    decompose_compose_equiv (U32.v v');
+    decompose_compare (U32.v v) (U32.v v')
+  in
+  let r0 = B.index b pos in
+  let r1 = B.index b (pos `U32.add` 1ul) in
+  let r2 = B.index b (pos `U32.add` 2ul) in
+  let r3 = B.index b (pos `U32.add` 3ul) in
+  [@inline_let] let b0 = U8.uint_to_t (decompose_int32_le_0 (U32.v v)) in
+  [@inline_let] let b1 = U8.uint_to_t (decompose_int32_le_1 (U32.v v)) in
+  [@inline_let] let b2 = U8.uint_to_t (decompose_int32_le_2 (U32.v v)) in
+  [@inline_let] let b3 = U8.uint_to_t (decompose_int32_le_3 (U32.v v)) in
+  compare_by_bytes r0 r1 r2 r3 b0 b1 b2 b3
+
+#pop-options
+
+inline_for_extraction
+let validate_constint32le
+  (v: U32.t { 0 <= U32.v v /\ U32.v v < 4294967296 } )
+: Tot (validator (parse_constint32le (U32.v v)))
+= fun #rrel #rel (input: slice rrel rel) (pos: U32.t) ->
+  let h = HST.get() in
+    let _ =
+      valid_constint32le (U32.v v) h input pos;    
+      valid_equiv (parse_int32_le ()) h input pos
+    in
+  if U32.lt (input.len `U32.sub` pos) 4ul
+  then
+    validator_error_not_enough_data
+  else
+    if inplace_compare v input pos then
+      pos `U32.add` 4ul
+    else
+      validator_error_generic
